\section{Geometric Brownian Motion}

Let $(X_t: t \ge 0)$ be a Brownian motion with constant drift on $\mbb{R}$ with generator

\begin{equation*}
    (\mathcal{L}f)(x) = \mu f'(x) + \frac{1}{2} \sigma^2 f''(x), \, \mu \in \mbb{R},\, \sigma > 0,
\end{equation*}

and initial condition $X_0 = 0$. \textbf{Geometric Brownian motion} is defined as

\begin{equation*}
    (Y_t: t \ge 0) \quad \text{with} \quad Y_t = e^{X_t}.
\end{equation*}

\begin{enumerate}
    \item[(a)] Show that $(Y_t: t \ge 0)$ is a diffusion process on $[0, \infty)$ and compute its generator. Write down the associated SDE and Fokker-Planck equation.

        \textit{ Sol. } Notice that 
        \begin{align}
            \E[(\mathcal{L}_Yf)(Y_t)] = & \frac{\dif}{\dif t} \E [f(Y_t)] \notag \\ 
            = & \frac{\dif}{\dif t} \E [f(e^{X_t})]. \label{eqn1}
        \end{align}
        Let $F = f \circ \exp$, then \eqref{eqn1} becomes
        \begin{align}
            \E[(\mathcal{L}_Yf)(Y_t)] = & \frac{\dif}{\dif t} \mbb{E} [f(e^{X_t})]  \notag \\ 
            = & \frac{\dif}{\dif t} \mbb{E} [F(X_t)] \notag \\ 
            = & \mbb{E} [(\mathcal{L}_X F)(X_t)]. \label{eqn2}
        \end{align}
        Since \eqref{eqn2} holds for all $f \in C^1{\mbb{R}}$, we know 
        \begin{align*}
            (\mathcal{L}_Yf)(Y_t) = & (\mathcal{L}_X F)(X_t) \\ 
            = & \mu \frac{\dif}{\dif x} f(e^{X_t}) + \frac{1}{2} \sigma^2 \frac{\dif ^2}{\dif x^2} f(e^{X_t}) \\ 
            = & \mu f'(e^{X_t}) e^{X_t} + \frac{1}{2} \sigma^2 \frac{\dif}{\dif x} ( f'(e^{X_t})e^{X_t}) \\ 
            = & \mu f'(e^{X_t}) e^{X_t} + \frac{1}{2} \sigma^2 (f''(e^{X_t})e^{2X_t} + f'(e^{X_t}) e^{X_t}) \\ 
            = & \mu f'(Y_t) Y_t + \frac{1}{2}\sigma^2 (f''(Y_t) Y_t^2 + f'(Y_t) Y_t) \\ 
            = & (\mu + \frac{1}{2} \sigma^2)Y_t f'(Y_t) + \frac{1}{2} (\sigma Y_t)^2 f''(Y_t),
        \end{align*}
        which shows $(Y_t: t \ge 0)$ is a diffusion process with the drift $(\mu + \frac{1}{2}\sigma^2) y$ and the diffusion $\sigma y$.

        \begin{eqnarray*}
            \lefteqn{\int_\mbb{R} \frac{\partial}{\partial t} p_t(x,y) f(y) \dif y} \\ 
            & = & \frac{\partial}{\partial t} \int_\mbb{R} p_t(x,y) f(y) \dif y \\ 
            & = & \frac{\partial}{\partial t} \E [f(Y_t)] \\ 
            & = & \E [(\mathcal{L}_Y f)(Y_t)] \\ 
            & = & \E \left[(\mu + \frac{1}{2} \sigma^2)Y_t f'(Y_t) + \frac{1}{2} (\sigma Y_t)^2 f''(Y_t)\right] \\ 
            & = & \int_\mbb{R} \left[ (\mu+\frac{1}{2}\sigma^2) y f'(y) + \frac{1}{2} (\sigma y)^2 f''(y) \right] p_t(x,y) \dif y \\ 
            & = & (\mu + \frac{1}{2} \sigma^2) \int_\mbb{R} y f'(y) p_t(x, y) \dif y + \frac{1}{2}\sigma^2 \int_\mbb{R} y^2 f''(y) p_t(x, y) \dif y \\ 
            & = &(\mu + \frac{1}{2} \sigma^2) \int_\mbb{R} y p_t(x,y) \dif f(y) + \frac{1}{2} \sigma^2 \int_\mbb{R} y^2 p_t(x,y) \dif f'(y) \\ 
            & = & (\mu + \frac{1}{2}\sigma^2) \left\{ \left. yp_t(x,y)f(y) \right|_{y = -\infty}^{y = \infty} - \int_\mbb{R} f(y) \left[p_t(x,y)+ y \frac{\partial}{\partial y} p_t(x, y)\right] \dif y\right\} \\ 
            & & + \frac{1}{2}\sigma^2 \left\{ \left. y^2p_t(x,y)f'(y) \right|_{y = -\infty}^{y = \infty} - \int_\mbb{R} f'(y) \left[ 2y p_t(x,y) + y^2 \frac{\partial}{\partial y} p_t(x,y) \right] \dif y\right\} \\ 
            & = & - (\mu + \frac{1}{2}\sigma^2)  \int_\mbb{R} f(y) \left[p_t(x,y)+ y \frac{\partial}{\partial y} p_t(x, y)\right] \dif y - \frac{1}{2} \sigma^2 \int_\mbb{R} f'(y) \left[ 2y p_t(x,y) + y^2 \frac{\partial}{\partial y} p_t(x,y) \right] \dif y \\ 
            & = & - (\mu + \frac{1}{2}\sigma^2)  \int_\mbb{R} f(y) \left[p_t(x,y)+ y \frac{\partial}{\partial y} p_t(x, y)\right] \dif y -  \frac{1}{2} \sigma^2 \int_\mbb{R} 2y p_t(x,y) + y^2 \frac{\partial}{\partial y} p_t(x,y) \dif f(y) \\ 
            & = & - (\mu + \frac{1}{2}\sigma^2)  \int_\mbb{R} f(y) \left[p_t(x,y)+ y \frac{\partial}{\partial y} p_t(x, y)\right] \dif y - \frac{1}{2} \sigma^2 \left\{ \left. [2y p_t(x,y) + y^2 \frac{\partial}{\partial y} p_t(x,y)] f(y) \right|_{y = -\infty}^{y = \infty} \right. \\ 
            & & \left. - \int_\mbb{R} f(y) [2p_t(x,y) + 4y \frac{\partial}{\partial y} p_t(x,y) + y^2 \frac{\partial^2}{\partial y^2} p_t(x,y)] \dif y \right\} \\ 
            & = & \int_\mbb{R} f(y) \left[ (\frac{1}{2}\sigma^2 - \mu) p_t(x,y) + (\frac{3}{2} \sigma^2 - \mu) y \frac{\partial}{\partial y} p_t(x,y) + \frac{1}{2}\sigma^2y^2\frac{\partial^2}{\partial y^2} p_t(x,y) \right] \dif y,
        \end{eqnarray*}
        so the Fokker-Planck equation is
        \begin{equation*}
            \frac{\partial}{\partial t} p_t(x,y) = (\frac{1}{2}\sigma^2 - \mu) p_t(x,y) + (\frac{3}{2} \sigma^2 - \mu) y \frac{\partial}{\partial y} p_t(x,y) + \frac{1}{2}\sigma^2y^2\frac{\partial^2}{\partial y^2} p_t(x,y).
        \end{equation*}

        An easier way is to use the conclusion for a diffusion process directly:
        \begin{align*}
            \frac{\partial}{\partial t} p_t(x,y) = & - \frac{\partial}{\partial y} \left[ (\mu + \frac{1}{2}\sigma^2) y p_t \right] + \frac{1}{2} \frac{\partial^2}{\partial y^2} \left(\sigma^2 y^2 p_t \right) \\ 
            = & - ( \mu + \frac{1}{2} \sigma^2) (p_t + y \frac{\partial}{\partial y}p_t(x,y)) + \frac{1}{2} \sigma^2 \frac{\partial}{\partial y} \left(2 y p_t + y^2 \frac{\partial}{\partial y} p_t(x,y) \right) \\ 
            = & (\frac{1}{2}\sigma^2 - \mu) p_t(x,y) + (\frac{3}{2} \sigma^2 - \mu) y \frac{\partial}{\partial y} p_t(x,y) + \frac{1}{2}\sigma^2y^2\frac{\partial^2}{\partial y^2} p_t(x,y).
        \end{align*}

        The associated SDE is 
        \begin{equation*}
            d Y_t = (\mu + \frac{1}{2}\sigma^2) Y_t \dif t + \sigma Y_t \dif B_t.
        \end{equation*}

    \item[(b)] Use the evolution equation of expectation values of test functions $f: \mbb{R} \to \mbb{R}$
    
        \begin{equation*}
            \frac{\dif}{\dif t} \mbb{E}[f(Y_t)] = \mbb{E}[\mathcal{L}f(Y_t)],
        \end{equation*}

        to derive ODEs for the meane $m(t) := \mathbb{E}[Y_t]$ and the second moment $m_2(t) := \mbb{E}[Y_t^2]$. (No need to solve the ODEs.)

        \textit{ Sol. }

    \item[(c)] Under which conditions on $\mu$ and $\sigma^2$ is $(Y_t: t \ge 0)$ a martingale? 
    
    What is the asymptotic behaviour of the variance $v(t) = m_2(t) - m(t)^2$ in that case?
    
        \textit{ Sol. }

    \item[(d)] Show that $\delta_0$ is the unique stationary distribution of the process on the state space $[0, \infty)$. Under which conditions on $\mu$ and $\sigma^2$ does the process with $Y_0 = 1$ converge to the stationary distribution?
    
    Under which conditions on $\mu$ and $\sigma^2$ is the process ergodic? Justify your answer.

        \textit{ Sol. }

    \item[(e)] For $\sigma^2 = 1$ choose $\mu = -1/2$ and two other values $\mu < -1/2$ and $\mu > 1/2$. Simulate and plot a sample path of the process with $Y_0 = 1$ up to time $t = 10$, by numerically integrating the corresponding SDE with time steps $\Delta t = 0.1$ and $0.01$.
    
        \textit{ Sol. }

\end{enumerate}